factor out essentials to CellularBase, rework Finite to use neighbourhoods, add remaining neighbourhood stuff to Toroidal

project/FiniteElementaryCellular.thy
@@ -3,11 +3,14 @@
 (*reference damien's cylinders for those *)
 
 theory FiniteElementaryCellular
-  imports Main
+  imports Main CellularBase
 begin
 
 section \<open>Basic definitions of Finite Elementary Cellular Automata\<close>
+(* Going to go with left/right boundaries as Zero by default *)
+(* Might like that to be flexible somehow? Without ruining CA type def*)
 
+(*
 (* might re-add width on a type level if it might help in proofs?*)
 datatype cell = One | Zero
 type_synonym state = "cell list"
@@ -17,18 +20,13 @@ type_synonym edge_rule = "cell \<Rightarrow> cell \<Rightarrow> cell"
 (* could merge all rules into one compositite type *)
 datatype CA = CA (State : state) (Rule : rule) (LeftRule : edge_rule)  (RightRule : edge_rule)
 
-definition null_rule :: rule where
-"null_rule _ _ _ = Zero"
+
 
 definition null_edge :: edge_rule where
 "null_edge _ _ = Zero"
+*)
 
-definition testCA :: CA where
-"testCA = CA [One, One, Zero] null_rule null_edge null_edge"
-
-definition width :: "CA \<Rightarrow> nat" where
-"width ca = length (State ca)"
-
+(*
 (* first is leftmost *)
 fun left_update :: "CA \<Rightarrow> cell" where
 "left_update ca = (LeftRule ca) ((State ca) ! 0) ((State ca) ! 1)"
@@ -38,27 +36,24 @@ fun right_update :: "CA \<Rightarrow> cell" where
 "right_update ca = (let n = (width ca)-1 in (RightRule ca) ((State ca) ! (n-1)) ((State ca) ! n))"
 
 fun inner_update :: "CA \<Rightarrow> nat \<Rightarrow> cell" where
-"inner_update (CA state rule _ _) n = rule (state ! (n-1)) (state ! n) (state ! (n+1))"
+"inner_update (CA state rule _ _) n = rule (state ! (n-1)) (state ! n) (state ! (n+1))" 
 
 fun update_cell :: "CA \<Rightarrow> nat \<Rightarrow> cell" where
 "update_cell ca 0 = left_update ca" |
-"update_cell ca n = (if n = ((width ca)-1) then right_update ca else inner_update ca n)"
+"update_cell ca n = (if n = ((width ca)-1) then right_update ca else inner_update ca n)"*)
 
+(*fun update_CA :: "CA \<Rightarrow> CA" where
+"update_CA ca = (CA (map (update_cell ca) [0..<width ca]) (Rule ca) (LeftRule ca) (RightRule ca))"*)
 
+fun nbhds :: "state \<Rightarrow> neighbourhood list" where
+"nbhds [] = []" | (*this should never happen*)
+"nbhds (x#xs) = ((Nb Zero x (hd xs)) # (inner_nbhds (x#xs))) @ [Nb (last (butlast xs)) (last xs) Zero]"
 
 fun update_CA :: "CA \<Rightarrow> CA" where
-"update_CA ca = (CA (map (update_cell ca) [0..<width ca]) (Rule ca) (LeftRule ca) (RightRule ca))"
-
-fun apply_t_times :: "('a \<Rightarrow> 'a) \<Rightarrow> 'a \<Rightarrow> nat \<Rightarrow> 'a" where
-"apply_t_times f a 0 = a" |
-"apply_t_times f a (Suc n) = apply_t_times f (f a) n"
+"update_CA (CA s r) = CA (map r (nbhds s)) r"
 
 fun run_t_steps :: "CA \<Rightarrow> nat \<Rightarrow> CA" where
 "run_t_steps ca n = apply_t_times update_CA ca n"
-
-
-(*definition yields :: "CA \<Rightarrow> state \<Rightarrow> bool" (infixr \<open>yields\<close>  65) where
-"A yields s = (\<exists> n. State (run_t_steps A n) = s)"*)
 
 definition yields :: "CA \<Rightarrow> state \<Rightarrow> bool" (infixr \<open>yields\<close>  65) where
 "A yields s \<equiv> (\<exists> n. State (run_t_steps A n) = s \<and> n > 0)"
@@ -66,22 +61,13 @@ definition yields :: "CA \<Rightarrow> state \<Rightarrow> bool" (infixr \<open>
 definition loops :: "CA \<Rightarrow> bool" where
 "loops ca \<equiv> ca yields State ca"
 
-definition wellformed :: "CA \<Rightarrow> bool" where
-"wellformed ca \<equiv> (width ca \<ge> 3)"
-
 (* maybe add some infix notation for this *)
 (* maybe change to run_t_steps 1 for more precision *)
 fun garden_of_eden :: "CA \<Rightarrow> bool" where
-"garden_of_eden (CA s rule l r) = (\<not>(\<exists> s0. (CA s0 rule l r) yields s))"
+"garden_of_eden (CA s r) = (\<not>(\<exists> s0. (CA s0 r) yields s))"
 
 fun reversible :: "CA \<Rightarrow> bool" where
-"reversible (CA _ rule l r) = (\<forall>s. (\<exists>!s0. State (run_t_steps (CA s0 rule l r) 1) = s))"
-
-
-(* Only valid for old definition *)
-(*theorem "ca yields State ca"
-  apply(metis State_def apply_t_times.simps(1) le_boolD order_refl run_t_steps.simps yields_def)
-  done*)
+"reversible (CA _ r) = (\<forall>s. (\<exists>!s0. State (update_CA (CA s0 r)) = s))"
 
 theorem "ca yields State (run_t_steps ca 1)"
 proof-
@@ -95,41 +81,11 @@ theorem t1 :"n>0 \<Longrightarrow> ca yields State (run_t_steps ca n)"
   apply(auto)
   done
 
-theorem
-  fixes ca :: CA
-  assumes wf : "wellformed ca"
-  shows "map (update_cell ca) [0..<width ca] = left_update ca # (map ) @ [right_update ca]"
-proof -
-qed
-
 
 theorem "testCA yields [Zero, Zero, Zero]"
   apply(simp add: yields_def)
   apply(rule_tac x=1 in exI)
   apply(rule conjI)
-  apply(auto)
-
-
-
-fun left_zero_pad :: "rule \<Rightarrow> cell \<Rightarrow> cell \<Rightarrow> cell" where
-"left_zero_pad rule c1 c2 = rule Zero c1 c2"
-
-fun right_zero_pad :: "rule \<Rightarrow> cell \<Rightarrow> cell \<Rightarrow> cell" where
-"right_zero_pad rule c2 c1 = rule c2 c1 Zero"
-
-fun rule110 :: rule where
-"rule110  One One One = Zero"   |
-"rule110  One One Zero = One"   |
-"rule110  One Zero One = One"   |
-"rule110  One Zero Zero = Zero" |
-"rule110  Zero One One = One"   |
-"rule110  Zero One Zero = One"  |
-"rule110  Zero Zero One = One"  |
-"rule110  Zero Zero Zero = Zero"
-
-definition CA110 :: CA where
-"CA110 \<equiv> CA [Zero, Zero, Zero, Zero, One] rule110 (left_zero_pad rule110) (right_zero_pad rule110)" 
-  
- 
-
+   apply(auto)
+  sorry
 end
