project/ToroidalElementaryCellular.thy
@@ -1,37 +1,35 @@
 (*reference damien's cylinders for these *)
 
 theory ToroidalElementaryCellular
-  imports Main
+  imports Main CellularBase
 begin
 
 section \<open>Basic definitions of Toroidal Elementary Cellular Automata\<close>
 
-(* factor out the core essentials to both the 1D CA *)
-
-(* perhaps typeclass them so well-formed works on both! *)
-
-(* maybe rename so I can compare them but probably not necessary! *)
-
-datatype cell = One | Zero
-type_synonym state = "cell list"
-type_synonym rule = "cell \<Rightarrow> cell \<Rightarrow> cell \<Rightarrow> cell"
-
-datatype CA = CA (State : state) (Rule : rule)
-
 (* Generate the neighbourhoods for each cell *)
-(* TODO this is the only function that needs to change to make different topologies!*)
-
-(* maybe define neighbourhoods as a type? *)
-(* still easy enough to work with, or just a tuple? *)
-fun inner_nbhds :: "state \<Rightarrow> state list" where
-"inner_nbhds (x#y#z#[]) = [x, y, z] # []" |
-"inner_nbhds (x#y#z#zs) = [x,y,z] # (inner_nbhds (y#z#zs))" |
+(* this is the only function that needs to change to make different topologies!*)
+fun inner_nbhds :: "state \<Rightarrow> neighbourhood list" where
+"inner_nbhds (x#y#z#[]) = (Nb x y z) # []" |
+"inner_nbhds (x#y#z#zs) = (Nb x y z) # (inner_nbhds (y#z#zs))" |
 "inner_nbhds _ = []" (* neighbourhoods aren't defined for \<le> 2 *)
 
-fun nbhds :: "state \<Rightarrow> state list" where
+fun nbhds :: "state \<Rightarrow> neighbourhood list" where
 "nbhds [] = []" | (*this should never happen*)
-"nbhds (x#xs) = (((last xs)#x#[hd xs]) # (inner_nbhds (x#xs))) @ [(last (butlast xs))#(last xs)#[x]]"
+"nbhds (x#xs) = ((Nb (last xs) x (hd xs)) # (inner_nbhds (x#xs))) @ [Nb (last (butlast xs)) (last xs) x]"
+
 
 fun update_CA :: "CA \<Rightarrow> CA" where
-"update_CA (CA s r) = CA (map update_cell (nbhds s)) r"
+"update_CA (CA s r) = CA (map r (nbhds s)) r"
+
+fun apply_t_times :: "('a \<Rightarrow> 'a) \<Rightarrow> 'a \<Rightarrow> nat \<Rightarrow> 'a" where
+"apply_t_times f a 0 = a" |
+"apply_t_times f a (Suc n) = apply_t_times f (f a) n"
+
+fun run_t_steps :: "CA \<Rightarrow> nat \<Rightarrow> CA" where
+"run_t_steps ca n = apply_t_times update_CA ca n"
+
+definition rule110 :: CA where
+"rule110 \<equiv> CA [Zero, One, Zero] r110" 
+
+value "State (run_t_steps rule110 5)"
 end
