project/CellularBase.thy
@@ -1,0 +1,65 @@
+theory CellularBase
+  imports Main
+begin
+
+section \<open>Base datatypes and definitions common to all Cellular Automata\<close>
+(* Might end up having different bases between 1 and 2D*)
+
+(* perhaps typeclass them so well-formed works on all? *)
+
+datatype cell = One | Zero
+type_synonym state = "cell list"
+datatype neighbourhood = Nb cell cell cell 
+type_synonym rule = "neighbourhood \<Rightarrow> cell"
+
+datatype CA = CA (State : state) (Rule : rule)
+
+definition width :: "CA \<Rightarrow> nat" where
+"width ca = length (State ca)"
+
+consts nbhds :: "state \<Rightarrow> neighbourhood list" (* This doesn't really do anything helpful yet *)
+
+(* 1D only *)
+fun inner_nbhds :: "state \<Rightarrow> neighbourhood list" where
+"inner_nbhds (x#y#z#[]) = (Nb x y z) # []" |
+"inner_nbhds (x#y#z#zs) = (Nb x y z) # (inner_nbhds (y#z#zs))" |
+"inner_nbhds _ = []" (* neighbourhoods aren't defined for \<le> 2 *)
+
+(*fun update_CA :: "CA \<Rightarrow> CA" where
+"update_CA (CA s r) = CA (map r (nbhds s)) r"*)
+
+definition null_rule :: rule where
+"null_rule _ = Zero"
+
+(*definition testCA :: CA where
+"testCA = CA [One, One, Zero] null_rule null_edge null_edge"*)
+
+fun apply_t_times :: "('a \<Rightarrow> 'a) \<Rightarrow> 'a \<Rightarrow> nat \<Rightarrow> 'a" where
+"apply_t_times f a 0 = a" |
+"apply_t_times f a (Suc n) = apply_t_times f (f a) n"
+
+definition wellformed :: "CA \<Rightarrow> bool" where
+"wellformed ca \<equiv> (width ca \<ge> 3)"
+
+(*definition yields :: "CA \<Rightarrow> state \<Rightarrow> bool" (infixr \<open>yields\<close>  65) where
+"A yields s \<equiv> (\<exists> n. State (run_t_steps A n) = s \<and> n > 0)"
+
+definition loops :: "CA \<Rightarrow> bool" where
+"loops ca \<equiv> ca yields State ca"
+
+fun garden_of_eden :: "CA \<Rightarrow> bool" where
+"garden_of_eden (CA s rule l r) = (\<not>(\<exists> s0. (CA s0 rule l r) yields s))"
+
+fun reversible :: "CA \<Rightarrow> bool" where
+"reversible (CA _ rule l r) = (\<forall>s. (\<exists>!s0. State (run_t_steps (CA s0 rule l r) 1) = s))"*)
+
+fun r110 :: rule where
+"r110  (Nb One One One) = Zero"   |
+"r110  (Nb One One Zero) = One"   |
+"r110  (Nb One Zero One) = One"   |
+"r110  (Nb One Zero Zero) = Zero" |
+"r110  (Nb Zero One One) = One"   |
+"r110  (Nb Zero One Zero) = One"  |
+"r110  (Nb Zero Zero One) = One"  |
+"r110  (Nb Zero Zero Zero) = Zero"
+end
